cava/Cava/Util/Tuple.v
@@ -1,0 +1,177 @@
+(****************************************************************************)
+(* Copyright 2021 The Project Oak Authors                                   *)
+(*                                                                          *)
+(* Licensed under the Apache License, Version 2.0 (the "License")           *)
+(* you may not use this file except in compliance with the License.         *)
+(* You may obtain a copy of the License at                                  *)
+(*                                                                          *)
+(*     http://www.apache.org/licenses/LICENSE-2.0                           *)
+(*                                                                          *)
+(* Unless required by applicable law or agreed to in writing, software      *)
+(* distributed under the License is distributed on an "AS IS" BASIS,        *)
+(* WITHOUT WARRANTIES OR CONDITIONS OF ANY KIND, either express or implied. *)
+(* See the License for the specific language governing permissions and      *)
+(* limitations under the License.                                           *)
+(****************************************************************************)
+
+Require Import Coq.Lists.List.
+
+Import ListNotations.
+
+Fixpoint curried (l: list Type) ret: Type :=
+  match l with
+  | [] => ret
+  | x::xs => x -> curried xs ret
+  end.
+
+Fixpoint tupled (l: list Type) prefix: Type :=
+  match l with
+  | [] => prefix
+  | x::xs => tupled xs (prefix * x)%type
+  end.
+
+Definition tupled' (l: list Type): Type :=
+  match l with
+  | [] => unit
+  | x::xs => tupled xs x
+  end.
+
+Fixpoint tupledR (l : list Type) : Type :=
+  match l with
+  | [] => unit
+  | x :: xs => x * tupledR xs
+  end.
+
+Definition uncurried' (l: list Type) ret: Type :=
+  tupledR l -> ret.
+  (* match l with *)
+  (* | [] => ret *)
+  (* | x::xs => uncurried xs x ret *)
+  (* end. *)
+
+Fixpoint unbalance (ts: list Type) {accumT : Type}
+  : tupled ts accumT -> accumT * tupledR ts :=
+  match ts with
+  | [] => fun acc => (acc, tt)
+  | x::xs => fun ab =>
+      let '(acc, vx, vxs) := unbalance xs ab in
+      (acc, (vx, vxs))
+  end.
+
+Definition unbalance' (ts : list Type)
+                     : tupled' ts -> tupledR ts :=
+  match ts with
+  | [] => fun _ => tt
+  | x::xs => unbalance xs
+  end.
+
+Fixpoint rebalance (ts : list Type) {accumT : Type} (accum : accumT)
+  : tupledR ts -> tupled ts accumT :=
+  match ts with
+  | [] => fun _ : unit => accum
+  | x::xs =>
+    fun ab => rebalance xs (accum, fst ab) (snd ab)
+  end.
+
+Definition rebalance' (ts : list Type)
+  : tupledR ts -> tupled' ts :=
+  match ts with
+  | [] => fun _ => tt
+  | x::xs => fun ab => rebalance xs (fst ab) (snd ab)
+  end.
+
+Fixpoint curry (l : list Type) ret {struct l}: uncurried' l ret -> curried l ret :=
+  match l with
+  | [] => fun f => f tt
+  | X :: XS => fun f x =>
+      curry XS ret (fun txs => f (x, txs))
+  end.
+
+Fixpoint curry_helper l ret {struct l}: (tupled' l -> ret) -> uncurried' l ret :=
+  match l with
+  | [] => fun f => f
+  | X::XS => fun f '(y,ys) => f (rebalance XS y ys)
+  end.
+
+Fixpoint uncurry (l : list Type) ret {struct l}: curried l ret -> uncurried' l ret :=
+  match l with
+  | [] => fun f _ => f
+  | X :: XS => fun f '(y,ys) => uncurry XS ret (f y) ys
+  end.
+
+
+
+(*     (1* forall prefix : Type, prefix -> curried l (tupled l prefix) := *1) *)
+
+(* Fixpoint curry_helper (l : list Type): *)
+(*     forall prefix : Type, prefix -> curried l (tupled l prefix) := *)
+(*   match l with *)
+(*   | [] => fun _ x => x *)
+(*   | X :: XS => *)
+(*       fun prefix (p: prefix) (x: X) => *)
+(*       curry_helper _ (prefix * X)%type (p, x) *)
+(*   end. *)
+
+(* Fixpoint curry_helper2 {o} (l : list Type): *)
+(*   forall prefix, (tupled l prefix -> o) -> curried l (tupled l prefix) -> curried l o := *)
+(*   match l with *)
+(*   | [] => fun prefix f (x : curried [] (tupled [] prefix)) => f x *)
+(*   | X :: XS => fun prefix f x y => *)
+(*     curry_helper2 XS (prefix * X)%type f (x y) *)
+(*   end. *)
+
+(* (1* Fixpoint uncurried_apply (l : list Type) (ret : Type): *1) *)
+(* (1*   forall prefix, tupled l prefix -> uncurried l prefix ret -> ret := *1) *)
+(* (1*   match l with *1) *)
+(* (1*   | [] => fun _ args f => f args *1) *)
+(* (1*   | X :: XS => fun prefix args f => *1) *)
+(* (1*     uncurried_apply XS ret (prefix * X) args f *1) *)
+(* (1*   end. *1) *)
+
+(* (1* Definition curry (l : list Type) ret: uncurried' l ret -> curried l ret := *1) *)
+(* (1*   match l with *1) *)
+(* (1*   | [] => fun x => x *1) *)
+(* (1*   | X::XS => fun f x => curry_helper2 _ X (fun y => uncurried_apply _ ret X y f) (curry_helper _ X x) *1) *)
+(* (1*   end. *1) *)
+
+(* (1* Fixpoint uncurried_helper (l : list Type) (ret : Type): *1) *)
+(* (1*   forall prefix, (tupled l prefix -> ret) -> uncurried l prefix ret := *1) *)
+(* (1*   match l with *1) *)
+(* (1*   | [] => fun _ f => f *1) *)
+(* (1*   | X :: XS => fun prefix f => uncurried_helper XS ret (prefix * X)%type f *1) *)
+(* (1*   end. *1) *)
+
+(* (1* Definition uncurried_helper' l ret: (tupled' l -> ret) -> uncurried' l ret := *1) *)
+(* (1*   match l with *1) *)
+(* (1*   | [] => fun f => f tt *1) *)
+(* (1*   | X::XS => fun f => uncurried_helper XS ret X f *1) *)
+(* (1*   end. *1) *)
+
+
+(* (1* Fixpoint curried_apply (l : list Type) (ret : Type) {struct l}: *1) *)
+(* (1*   forall p, tupledR p -> curried l ret -> ret. *1) *)
+(* (1* destruct l; intros. *1) *)
+(* (1* exact X0. *1) *)
+(* (1* eapply curried_apply. *1) *)
+(* (1* apply X. *1) *)
+(* (1* apply X0. *1) *)
+(* (1* Defined. *1) *)
+
+
+
+(* (1* exact X0. *1) *)
+
+(* (1* eapply curried_apply. *1) *)
+(* (1* apply X. *1) *)
+(* (1* apply X. *1) *)
+(* (1* apply X0. *1) *)
+(* (1* destruct l. *1) *)
+
+(* (1*   match l *1) *)
+(* (1*   as l return *1) *)
+(* (1*   forall prefix, tupled l prefix -> curried l ret -> ret *1) *)
+(* (1*   with *1) *)
+(* (1*   | [] => fun _ args f => f *1) *)
+(* (1*   | X :: XS => fun prefix '((y,ys) : tupled (X :: XS) _) f => *1) *)
+(* (1*     curried_apply XS ret (prefix * X) ys (f y) *1) *)
+(* (1*   end. *1) *)
